examples/SchnorrPK.ec
@@ -109,29 +109,17 @@ section SchnorrPKSecurity.
   (* Completeness *)
   lemma schnorr_proof_of_knowledge_completeness_ll:
     islossless Completeness(SchnorrPK).main.
-  proof.
-    proc; inline*.
-    wp; rnd; wp; rnd; wp; skip; progress by apply FDistr.dt_ll.
-  qed.
-
+  proof. by islossless; apply FDistr.dt_ll. qed.
 
   lemma schnorr_proof_of_knowledge_completeness h w' &m:
     R h w' =>
     Pr[Completeness(SchnorrPK).main(h, w') @ &m : res] = 1%r.
   proof.
     rewrite /R /R_DL; move => sigmarel.
-    byphoare (_: h = x /\ w' = w ==> _) => //.
+    byphoare (_: h = x /\ w' = w ==> _) => //; rewrite sigmarel.
     proc; inline*; swap 3 -2; swap 8 -7.
-    wp; rewrite /snd /=.
-    rnd; rnd; skip.
-    progress => //. subst x{hr}.
-    have <-/=: predT = fun x => mu FDistr.dt (fun (x0 : t) => g ^ x0 * g ^ w{hr} ^ x = g ^ (x0 + x * w{hr})) = 1%r.
-      rewrite fun_ext => x; rewrite muE /=.
-      have ->/=: (fun (x0 : t) => if g ^ x0 * g ^ w{hr} ^ x = g ^ (x0 + x * w{hr}) then mass FDistr.dt x0 else 0%r) = (fun x0 => mass FDistr.dt x0).
-        rewrite fun_ext => z.
-        have ->//: g ^ z * g ^ w{hr} ^ x = g ^ (z + x * w{hr}) by rewrite pow_pow mul_pow mulC //.
-      rewrite -weightE FDistr.dt_ll /predT //.
-    rewrite FDistr.dt_ll //.
+    wp; rewrite /snd /=; auto => &hr />.
+    rewrite FDistr.dt_ll => /> *; algebra.
   qed.
 
   (* Special soundness *)
@@ -141,27 +129,15 @@ section SchnorrPKSecurity.
     g^r' = msg*(h^ch') =>
     Pr[SpecialSoundnessExperiment(SchnorrPK, SchnorrPKAlgorithms).main(h, msg, ch, r, ch', r') @ &m : (res <> None /\ R h (oget res))] = 1%r.
   proof.
-    move => challenges_differ.
-    move => accepting_transcript_1.
-    move => accepting_transcript_2.
+    move => challenges_differ
+            accepting_transcript_1
+            accepting_transcript_2.
     byphoare (_: h = x /\ msg = m /\ ch = e /\ ch' = e' /\ r = z /\ r' = z' ==> _) => //.
     proc; simplify; inline*.
-    auto; rewrite /R /R_DL /oget.
-    move => &hr [_] [_] [_] [_] [_] _; subst.
-    rewrite challenges_differ accepting_transcript_1 accepting_transcript_2 /=.
-    have algebra_part1 : (g ^ z{hr} / (g ^ z'{hr}) = m{hr} * x{hr} ^ e{hr} / m{hr} / x{hr} ^ e'{hr}).
-      rewrite accepting_transcript_1 accepting_transcript_2.
-      rewrite -3!div_def log_gpow -pow_bij 2!log_mul.
-      rewrite sub_def -oppfD addA -2!sub_def //.
-    have algebra_part2 : (g ^ z{hr} / (g ^ z'{hr}) = x{hr} ^ e{hr} / (x{hr} ^ e'{hr})).
-      rewrite algebra_part1.
-      rewrite -3!div_def log_gpow -pow_bij log_mul.
-      rewrite addC 2!sub_def addC -addA addfN addf0 addC -sub_def //.
-    have algebra_part3 : g ^ z{hr} / g ^ z'{hr} = g ^ z{hr} * g ^ -z'{hr}.
-      rewrite pow_opp inv_def -div_def 2!log_pow sub_def -mul_pow -pow_pow gpow_log //.
-    have ->//: x{hr} = g ^ ((z{hr} - z'{hr}) / (e{hr} - e'{hr})).
-      rewrite div_def 2!sub_def -pow_pow -mul_pow -algebra_part3 algebra_part2.
-      rewrite -div_def pow_pow 2!log_pow sub_def; algebra.
+    auto; rewrite /R /R_DL /oget => &hr /> ? 2!-> /=.
+    rewrite F.div_def -pow_pow F.sub_def -mul_pow pow_opp log_bij.
+    rewrite accepting_transcript_1 accepting_transcript_2 !(log_gpow, log_pow, log_mul, inv_def). 
+    by field; apply: contra H => heq; ring heq.
   qed.
 
   (* Special honest verifier zero knowledge *)
@@ -169,32 +145,20 @@ section SchnorrPKSecurity.
     Pr[SimulateHonestVerifier(SchnorrPK, SchnorrPKAlgorithms, D).gameIdeal() @ &m : res] = 
     Pr[SimulateHonestVerifier(SchnorrPK, SchnorrPKAlgorithms, D).gameReal() @ &m : res].
   proof.
-    move : FDistr.dt_ll FDistr.dt_fu FDistr.dt1E; rewrite /is_full => dt_ll dt_fu dt_supp.
+  (*  move : FDistr.dt_ll FDistr.dt_fu FDistr.dt1E; rewrite /is_full => dt_ll dt_fu dt_supp. *)
     byequiv => //.
     proc; inline*.
-    seq 27 22: ((glob D){1} = (glob D){2} /\ i{1} = 0 /\ x{1} = h{1} /\ x{2} = h{2} /\ to{1} = Some t{2} /\ ={h, w, e}).
-    swap{1} 15 -7; swap{2} 12 -5; swap{1} 11 -3; wp.
-    (* Let's play with randomness... *)
-    rnd (fun z, z - w{1}*e{1}) (fun r, r + w{1}*e{1}).
-    rnd; rnd{1}; wp; rnd; skip; progress => //.
-    + rewrite mulN1f sub_def -addA oppK (addC _ eL) -sub_def subff addf0 //.
-    + rewrite 2!dt_supp //.
-    + rewrite dt_fu //.
-    + rewrite mulN1f sub_def -addA oppK -sub_def subff addf0 //.
-    + algebra.
-    + algebra.
-    + rewrite mulN1f sub_def -addA oppK mulC mulN1f -sub_def subff addf0 //.
-    + rewrite sub_def -addA -sub_def subff addf0 //.
-    + rewrite 2!dt_supp //.
-    + rewrite dt_fu //.
-    + rewrite sub_def -addA (addC _ (w0L * eL)) -sub_def subff addf0 //.
-    + algebra.
-    + algebra.
-    + rewrite sub_def -addA mulC (addC _ (eL * w0L)) -sub_def subff addf0 //.
-    seq 2 0 : ((glob D){1} = (glob D){2} /\ ={x, t}); wp.
-    while{1} (to{1} = Some t{2}) (i{1}); progress.
-    wp; rnd; wp; skip; progress.
-    call (_: true); simplify; skip; progress.
+    seq 27 22: ((glob D){1} = (glob D){2} /\ i{1} = 0 /\ x{1} = h{1} /\ x{2} = h{2} /\ 
+                 to{1} = Some t{2} /\ ={h, w, e}).
+    + swap{1} 15 -7; swap{2} 12 -5; swap{1} 11 -3; wp.
+      (* Let's play with randomness... *)
+      rnd (fun z, z - w{1}*e{1}) (fun r, r + w{1}*e{1}).
+      seq 2 2 : (#pre  /\ ={w0}); auto => /> &2; rewrite FDistr.dt_ll /de /=.
+      move=> r1 _ eL _ _.
+      split => [rR _ | _]; 1: by ring.
+      split => [rR _ | _ z1L _]; 1: by rewrite !FDistr.dt1E.
+      by rewrite FDistr.dt_fu /=; progress; algebra.
+    by call (_:true); rcondf{1} 1; auto.
   qed.
   (* The above three theorems prove that the Schnorr proof of knowledge is a Sigma protocol *)
 
